Finish scoping theorems for nameless names

src/Scoping.v
@@ -143,8 +143,8 @@ Unshelve. simpl. lia.
 Qed.
 
 Theorem scoped_ignores_sub : forall Γ,
-  (forall e, VAL Γ ⊢ e -> forall ξ, subst_preserves Γ ξ -> subst ξ e = e) /\
-  (forall e, EXP Γ ⊢ e -> forall ξ, subst_preserves Γ ξ -> subst ξ e = e).
+  (forall e, VAL Γ ⊢ e -> forall ξ, subst_preserves Γ ξ -> e.[ξ] = e) /\
+  (forall e, EXP Γ ⊢ e -> forall ξ, subst_preserves Γ ξ -> e.[ξ] = e).
 Proof.
   apply scoped_ind.
   * intros. reflexivity.
@@ -176,6 +176,10 @@ Corollary vclosed_ignores_sub :
 Proof.
   intros. pose (scoped_ignores_sub 0). destruct a. apply H0; auto.
 Qed.
+
+Hint Resolve eclosed_ignores_sub.
+
+Hint Resolve vclosed_ignores_sub.
 
 Theorem scope_ext : forall Γ,
   (forall e, VAL Γ ⊢ e ->  VAL (S Γ) ⊢ e) /\
@@ -427,6 +431,16 @@ Proof.
   * simpl. apply H0. lia.
 Qed.
 
+Lemma consn_scope : forall (vals : list Exp) Γ Γ' (ξ : Substitution),
+    Forall (fun v => VAL Γ' ⊢ v) vals ->
+    SUBSCOPE Γ ⊢ ξ ∷ Γ' ->
+    SUBSCOPE length vals + Γ ⊢ fold_right (fun v acc => v .: acc) ξ vals ∷ Γ'.
+Proof.
+  induction vals; intros.
+  * simpl. auto.
+  * simpl. inversion H. apply cons_scope; auto.
+Qed.
+
 Hint Resolve cons_scope.
 
 (** Substitution is scope-preserving. *)
@@ -548,60 +562,87 @@ Module SUB_IMPLIES_SCOPE.
     repeat destruct Compare_dec.lt_dec; auto; lia.
   Qed.
 
+  Lemma upn_magic : forall n Γ Γ', upn n (magic_ξ Γ Γ') = magic_ξ (n + Γ) (n + Γ').
+  Proof.
+    induction n; intros; simpl; auto.
+    rewrite <- up_magic, IHn. auto.
+  Qed.
+
   Lemma magic_ξ_implies_scope : forall e Γ Γ',
       (EXP Γ' ⊢ e.[magic_ξ Γ Γ'] ->
        EXP Γ ⊢ e) /\
       (VAL Γ' ⊢ e.[magic_ξ Γ Γ'] ->
        VAL Γ ⊢ e).
   Proof.
-    induction e;
-      intros Γ Γ';
-      split;
+    induction e using Exp_ind2 with
+    (Q := fun l =>
+      Forall (fun e => forall Γ Γ', (EXP Γ' ⊢ e.[magic_ξ Γ Γ'] ->
+       EXP Γ ⊢ e) /\
+      (VAL Γ' ⊢ e.[magic_ξ Γ Γ'] ->
+       VAL Γ ⊢ e)) l);
+      try intros Γ Γ';
+      try split;
       intros;
-      cbn in H;
-      try invert_scoped H;
-      try solve
-          [constructor;
-           let e := match goal with
-                    | [ |- EXP _ ⊢ ?e ] => e
-                    | [ |- VAL _ ⊢ ?e ] => e
-                    end in
-           match goal with
-           | [IHe : forall (Γ Γ' : Env), (_ -> EXP Γ ⊢ e) /\ (_ -> VAL Γ ⊢ e),
-                H : VAL _ ⊢ e.[magic_ξ Γ Γ'] |- _ ] =>
-             eapply IHe in H; try eassumption; auto
-           | [IHe : forall (Γ Γ' : Env), (_ -> EXP Γ ⊢ e) /\ (_ -> VAL Γ ⊢ e),
-                H : EXP _ ⊢ e.[magic_ξ Γ Γ'] |- _ ] =>
-             eapply IHe in H; try eassumption; auto
-           end];
-    auto.
-    - cbn in *.
-      unfold magic_ξ in H.
-      repeat destruct lt_dec;
-        auto.
-      inversion H; subst.
-      inversion H0.
-      auto.
-    - cbn in *.
-      unfold magic_ξ in H.
-      repeat destruct lt_dec;
-        auto.
-      inversion H.
-      auto.
-    - constructor.
-      constructor.
-      eapply IHe.
-      rewrite <- up_magic.
-      eauto.
-    - constructor.
-      eapply IHe.
-      rewrite <- up_magic.
-      eauto.
-    - constructor;
-        firstorder idtac.
-      eapply IHe0.
-      rewrite <- up_magic.
-      eauto.
+      try cbn in H.
+    1-2, 4, 6, 8: constructor.
+    constructor.
+    * break_match_hyp; 
+       (unfold magic_ξ in Heqs; break_match_hyp; [ auto | try congruence ]).
+       inversion H. inversion H0. subst. inversion Heqs. subst. lia.
+    * break_match_hyp; 
+       (unfold magic_ξ in Heqs; break_match_hyp; [ auto | try congruence ]).
+       inversion H. inversion H0. subst. inversion Heqs. subst. lia.
+    * inversion H. inversion H0. subst.
+      eapply IHe. rewrite upn_magic in H1. eauto.
+    * constructor. constructor. break_match_hyp; 
+       (unfold magic_ξ in Heqs; break_match_hyp; [ auto | try congruence ]).
+       inversion H. inversion H0. subst. inversion Heqs. subst. lia.
+    * constructor. constructor. break_match_hyp; 
+       (unfold magic_ξ in Heqs; break_match_hyp; [ auto | try congruence ]).
+       inversion H. inversion H0. subst. inversion Heqs. subst. lia.
+    * constructor. constructor. inversion H. inversion H0. subst.
+      eapply IHe. replace (up_subst (upn (Datatypes.length vl) (magic_ξ Γ Γ'))) with
+                          (upn (S (length vl)) ((magic_ξ Γ Γ'))) in H3 by reflexivity.
+      rewrite upn_magic in H3. eauto.
+    * constructor. constructor. inversion H. inversion H0. subst.
+      eapply IHe. replace (up_subst (upn (Datatypes.length vl) (magic_ξ Γ Γ'))) with
+                          (upn (S (length vl)) ((magic_ξ Γ Γ'))) in H3 by reflexivity.
+      rewrite upn_magic in H3. eauto.
+    * constructor. inversion H. subst.
+      eapply IHe. replace (up_subst (upn (Datatypes.length vl) (magic_ξ Γ Γ'))) with
+                          (upn (S (length vl)) ((magic_ξ Γ Γ'))) in H1 by reflexivity.
+      rewrite upn_magic in H1. eauto.
+    * inversion H. 2: inversion H0. constructor.
+      - eapply IHe; eauto.
+      - replace (ELit 0) with (subst (magic_ξ Γ Γ') (ELit 0)) in H3 by reflexivity.
+        intros. erewrite <- map_length in H4. specialize (H3 i H4).
+        rewrite map_nth in H3. subst. rewrite indexed_to_forall in IHe0.
+        rewrite map_length in H4.
+        eapply IHe0; eauto.
+    * inversion H.
+    * inversion H. 2: inversion H0. subst. constructor.
+      - eapply IHe1; eauto.
+      - eapply IHe2; eauto. rewrite up_magic in H4. eauto.
+    * inversion H.
+    * inversion H. 2: inversion H0. constructor.
+      - eapply IHe1; eauto.
+        replace (up_subst (upn (Datatypes.length vl) (magic_ξ Γ Γ'))) with
+                (upn (S (length vl)) (magic_ξ Γ Γ')) in H2 by reflexivity.
+        rewrite upn_magic in H2. exact H2.
+      - eapply IHe2; eauto.
+        rewrite up_magic in H5. exact H5.
+    * inversion H.
+    * inversion H. 2: inversion H0. constructor.
+      - eapply IHe1; eauto.
+      - eapply IHe2; eauto.
+    * inversion H.
+    * inversion H. 2: inversion H0. constructor.
+      - eapply IHe1; eauto.
+      - eapply IHe2; eauto.
+      - eapply IHe3; eauto.
+    * inversion H.
+    * constructor; auto.
+    * constructor.
   Qed.
 
   Lemma sub_implies_scope_exp : forall e Γ Γ',
@@ -624,7 +665,7 @@ Module SUB_IMPLIES_SCOPE.
     apply magic_ξ_scope.
   Qed.
 
-  Definition magic_ξ_2 Γ' :=
+(*   Definition magic_ξ_2 Γ' :=
     fun n =>
       if lt_dec n Γ'
       then Var n
@@ -734,58 +775,41 @@ Module SUB_IMPLIES_SCOPE.
       eapply magic_ξ_implies_scope.
     destruct (bar e).
     rewrite H1; auto.
-  Qed.
+  Qed. *)
 End SUB_IMPLIES_SCOPE.
 
 Definition sub_implies_scope_exp := SUB_IMPLIES_SCOPE.sub_implies_scope_exp.
 Definition sub_implies_scope_val := SUB_IMPLIES_SCOPE.sub_implies_scope_val.
-Definition sub_implies_scope_exp_1 := SUB_IMPLIES_SCOPE.sub_implies_scope_exp_1.
-Definition sub_implies_scope_val_1 := SUB_IMPLIES_SCOPE.sub_implies_scope_val_1.
+(* Definition sub_implies_scope_exp_1 := SUB_IMPLIES_SCOPE.sub_implies_scope_exp_1.
+Definition sub_implies_scope_val_1 := SUB_IMPLIES_SCOPE.sub_implies_scope_val_1. *)
 
-Lemma upn_Var : forall (Γ : Env) (ξ : var -> Expr) (v : var),
-    v < Γ -> upn Γ ξ v = Var v.
+Lemma upn_Var : forall (Γ : nat) (ξ : Substitution) (v : nat),
+    v < Γ -> upn Γ ξ v = inr v.
 Proof.
   intros Γ ξ.
   induction Γ;
     intros.
-  + auto.
-  + rewrite iterate_S.
-    destruct v;
-      asimpl;
-      auto.
-    rewrite IHΓ;
-      auto.
+  + inversion H.
+  + simpl. destruct v.
+    * simpl. auto.
+    * simpl. rewrite IHΓ. 2: lia. auto.
 Qed.
 
-Lemma scoped_ignores_sub : forall e Γ ξ,
+Corollary upn_ignores_sub : forall e Γ ξ,
      (EXP Γ ⊢ e -> e.[upn Γ ξ] = e) /\
      (VAL Γ ⊢ e -> e.[upn Γ ξ] = e).
 Proof.
-  induction e;
-    cbn;
-    split;
-    intros;
-    invert_scoped H;
-    auto using upn_Var;
-    try solve
-        [repeat
-           match goal with
-           | [ IHe : forall (Γ : Env) (ξ : var -> Expr), (EXP Γ ⊢ ?e -> _) /\ (VAL Γ ⊢ ?e -> _),
-                 H : VAL _ ⊢ ?e
-                 |- _] => eapply IHe in H
-           | [ IHe : forall (Γ : Env) (ξ : var -> Expr), (EXP Γ ⊢ ?e -> _) /\ (VAL Γ ⊢ ?e -> _),
-                 H : EXP _ ⊢ ?e
-                 |- _] => eapply IHe in H
-           end;
-         f_equal;
-         eauto].
+  intros. split; intros.
+  * eapply scoped_ignores_sub; eauto. intro. intros. apply upn_Var. auto.
+  * pose (scoped_ignores_sub Γ). destruct a. apply H0. auto.
+    intro. intros. apply upn_Var. auto.
 Qed.
 
 Lemma escoped_ignores_sub : forall e Γ ξ,
     EXP Γ ⊢ e -> e.[upn Γ ξ] = e.
-Proof.  
+Proof.
   intros.
-  eapply scoped_ignores_sub in H.
+  eapply upn_ignores_sub in H.
   eauto.
 Qed.
 Hint Resolve escoped_ignores_sub.
@@ -794,33 +818,13 @@ Lemma vscoped_ignores_sub : forall e Γ ξ,
     VAL Γ ⊢ e -> e.[upn Γ ξ] = e.
 Proof.
   intros.
-  eapply scoped_ignores_sub in H.
+  eapply upn_ignores_sub in H.
   eauto.
 Qed.
 Hint Resolve vscoped_ignores_sub.
 
-Lemma eclosed_ignores_sub : forall e ξ,
-     ECLOSED e -> e.[ξ] = e.
-Proof.
-  intros.
-  replace (e.[ξ]) with (e.[upn 0 ξ])
-    by (rewrite upn0; auto).
-  auto.
-Qed.
-Hint Resolve eclosed_ignores_sub.
-
-Lemma vclosed_ignores_sub : forall e ξ,
-     VCLOSED e -> e.[ξ] = e.
-Proof.
-  intros.
-  replace (e.[ξ]) with (e.[upn 0 ξ])
-    by (rewrite upn0; auto).
-  auto.
-Qed.
-Hint Resolve vclosed_ignores_sub.
-
 Lemma eclosed_sub_closed : forall v ξ,
-    ECLOSED v -> ECLOSED v.[ξ].
+    EXPCLOSED v -> EXPCLOSED v.[ξ].
 Proof.
   intros.
   rewrite eclosed_ignores_sub;
@@ -829,7 +833,7 @@ Qed.
 Hint Resolve eclosed_sub_closed.
 
 Lemma vclosed_sub_closed : forall v ξ,
-    VCLOSED v -> VCLOSED v.[ξ].
+    VALCLOSED v -> VALCLOSED v.[ξ].
 Proof.
   intros.
   rewrite vclosed_ignores_sub;
@@ -837,939 +841,30 @@ Proof.
 Qed.
 Hint Resolve vclosed_sub_closed.
 
-(* Continuations *)
-
-Inductive Kont : Type :=
-| Knil : Kont
-| Kcons : Expr -> Kont -> Kont.
-
-Infix "-:" := Kcons (at level 60, right associativity).
-
-Lemma Kont_eq_dec : forall (K K' : Kont),
-    decidable (K = K').
-Proof.
-  unfold decidable.
-  induction K;
-    destruct K';
-    intros;
-    try solve [intuition auto].
-  destruct (Expr_eq_dec e e0);
-    subst;
-    revgoals.
-  { right.
-    contradict n.
-    inversion n; subst; auto.
-  }
-  specialize (IHK K').
-  inversion IHK; subst.
-  + left; auto.
-  + right.
-    contradict H.
-    inversion H.
-    auto.
-Qed.
-
-Reserved Notation "'KCLOSED' K" (at level 69).
-
-Inductive KontScoped : forall K, Prop :=
-| KontScoped_nil :
-    KCLOSED Knil
-| KontScoped_cons : forall K e,
-    EXP 1 ⊢ e ->
-    KCLOSED K ->
-    KCLOSED e -: K
-where
-"'KCLOSED' K" := (KontScoped K).
-
-Hint Constructors KontScoped.
-
-Theorem var_not_closed1 n v : ~ VALCLOSED (EVar n v).
-Proof. intro. inversion H. inversion H1. Qed.
-
-Hint Resolve var_not_closed1.
-
-Theorem var_not_closed2 n v : ~ EXPCLOSED (EVar n v).
-Proof. intro. inversion H. eapply var_not_closed1. eauto. Qed.
-
-Hint Resolve var_not_closed2.
-
-Theorem funid_not_closed1 n f : ~ VALCLOSED (EFunId n f).
-Proof. intro. inversion H. inversion H1. Qed.
-
-Hint Resolve funid_not_closed1.
-
-Theorem funid_not_closed2 n f : ~ EXPCLOSED (EFunId n f).
-Proof. intro. inversion H. eapply funid_not_closed1. eauto. Qed.
-
-Hint Resolve funid_not_closed2.
-
-(* Theorem restrict_in : forall l ξ v,
-  In v l -> (ξ -- l) v = idsubst v.
-Proof.
-  intros. unfold "--". apply in_list_sound in H. rewrite H. auto.
-Qed.
-
-Theorem restrict_not_in : forall l ξ v,
-  ~In v l -> (ξ -- l) v = ξ v.
-Proof.
-  intros. unfold "--". apply not_in_list_sound in H. rewrite H. auto.
-Qed. *)
-
-
-
-
-Theorem subscoped_preserves_app : forall ξ Γ Γ',
-  subscoped Γ Γ' ξ -> (subscoped (S Γ) (S Γ') (up_subst ξ)).
-Proof.
-  intros. intro. intros. break_match_goal.
-  * unfold subscoped in H.
-Qed.
-
-Hint Resolve subscoped_preserves_app.
-
-Corollary subscoped_ext :
-  forall ξ Γ Γ' l, subscoped (Γ ++ l) Γ' ξ -> subscoped Γ Γ' ξ.
-Proof.
-  unfold subscoped. intros. intuition.
-Qed.
-
-Theorem subst_restrict_comm : forall ξ l1 l2,
-  (ξ -- l1 -- l2) = (ξ -- l2 -- l1).
-Proof.
-  intros. unfold "--". extensionality x.
-  repeat break_match_goal; auto.
-Qed.
-
-Theorem subst_remove_scope : forall e Γ ξ l,
-  (EXP Γ ⊢ subst ξ e -> EXP Γ ++ l ⊢ subst (ξ -- l) e) /\
-  (VAL Γ ⊢ subst ξ e -> VAL Γ ++ l ⊢ subst (ξ -- l) e).
-Proof.
-  induction e using Exp_ind2 with 
-    (Q := fun l => Forall (fun e => forall Γ ξ l,
-  (EXP Γ ⊢ subst ξ e -> EXP Γ ++ l ⊢ subst (ξ -- l) e) /\
-  (VAL Γ ⊢ subst ξ e -> VAL Γ ++ l ⊢ subst (ξ -- l) e)) l)
-  ; try split; intros.
-  * repeat constructor.
-  * repeat constructor.
-  * unfold subst. destruct (in_dec var_funid_eq_dec (inl v) l) eqn:P.
-    - rewrite restrict_in by auto. simpl. constructor. constructor. intuition.
-    - rewrite restrict_not_in by auto. unfold subst in H. apply scope_ext_app. auto.
-  * unfold subst. destruct (in_dec var_funid_eq_dec (inl v) l) eqn:P.
-    - rewrite restrict_in by auto. simpl. constructor. intuition.
-    - rewrite restrict_not_in by auto. unfold subst in H. apply scope_ext_app. auto.
-  * unfold subst. destruct (in_dec var_funid_eq_dec (inr f) l) eqn:P.
-    - rewrite restrict_in by auto. simpl. constructor. constructor. intuition.
-    - rewrite restrict_not_in by auto. unfold subst in H. apply scope_ext_app. auto.
-  * unfold subst. destruct (in_dec var_funid_eq_dec (inr f) l) eqn:P.
-    - rewrite restrict_in by auto. simpl. constructor. intuition.
-    - rewrite restrict_not_in by auto. unfold subst in H. apply scope_ext_app. auto.
-  * simpl. constructor. constructor.
-    rewrite <- app_assoc. pose (perm_scoped (Γ ++ map inl vl ++ l)). destruct a.
-    clear H0. apply H1. rewrite subst_restrict_comm. rewrite app_assoc. apply IHe.
-    inversion H. inversion H0. subst. auto.
-    apply Permutation_app; auto. apply Permutation_app_comm.
-  * simpl. constructor.
-    rewrite <- app_assoc. pose (perm_scoped (Γ ++ map inl vl ++ l)). destruct a.
-    clear H0. apply H1. rewrite subst_restrict_comm. rewrite app_assoc. apply IHe.
-    inversion H. subst. auto.
-    apply Permutation_app; auto. apply Permutation_app_comm.
-  * simpl. constructor. constructor.
-    rewrite <- app_assoc. pose (perm_scoped (Γ ++ (inr f :: map inl vl) ++ l)).
-    destruct a.
-    clear H0. apply H1. rewrite subst_restrict_comm. rewrite app_assoc. apply IHe.
-    inversion H. inversion H0. subst. auto.
-    apply Permutation_app; auto. apply Permutation_app_comm.
-  * simpl. constructor.
-    rewrite <- app_assoc. pose (perm_scoped (Γ ++ (inr f :: map inl vl) ++ l)).
-    destruct a.
-    clear H0. apply H1. rewrite subst_restrict_comm. rewrite app_assoc. apply IHe.
-    inversion H. subst. auto.
-    apply Permutation_app; auto. apply Permutation_app_comm.
-  * inversion H. 2: inversion H0. simpl. constructor.
-    - apply IHe. auto.
-    - rewrite indexed_to_forall in IHe0. intros.
-      replace (ELit 0) with (subst (ξ -- l) (ELit 0)) by reflexivity.
-      rewrite map_nth. apply IHe0. rewrite map_length in H4. auto.
-      rewrite map_length in H4. erewrite <- map_length in H4. specialize (H3 i H4).
-      replace (ELit 0) with (subst ξ (ELit 0)) in H3 by reflexivity.
-      rewrite map_nth in H3. auto.
-  * inversion H.
-  * inversion H. 2: inversion H0. subst.
-    simpl. constructor.
-    - apply IHe1. auto.
-    - rewrite <- app_assoc. eapply perm_scoped. rewrite subst_restrict_comm.
-      apply IHe2. eauto.
-      rewrite <- app_assoc. apply Permutation_app; auto. apply Permutation_app_comm.
-  * inversion H.
-  * inversion H. 2: inversion H0. subst.
-    simpl. constructor; rewrite subst_restrict_comm.
-    - rewrite <- app_assoc. eapply perm_scoped. apply IHe1. eauto.
-      rewrite <- app_assoc. apply Permutation_app; auto. apply Permutation_app_comm.
-    - rewrite <- app_assoc. eapply perm_scoped. apply IHe2. eauto.
-      rewrite <- app_assoc. apply Permutation_app; auto. apply Permutation_app_comm.
-  * inversion H.
-  * inversion H. subst. simpl.
-    constructor; [ apply IHe1 | apply IHe2 ]; auto.
-    inversion H0.
-  * inversion H.
-  * inversion H. subst. simpl.
-    constructor; [ apply IHe1 | apply IHe2 | apply IHe3 ]; auto.
-    inversion H0.
-  * inversion H.
-  * constructor; eauto.
-  * constructor.
-Qed.
-
-Definition vals_subscoped vals Γ :=
-  forall v, In v vals -> VAL Γ ⊢ v
-.
-
-(* 
-!!!!!!!!!!!!!
-This does not hold: 
-
-Theorem ex_subst_exp :
-  forall e ξ l vals, subst (ξ[[ l ::== vals ]]) e =
-              subst (idsubst [[l ::== vals]]) (subst ξ e).
-Proof.
-  intros. induction e.
-  * simpl. reflexivity.
-  * simpl. *)
-(*
-This does not hold:
-
-bc. e ::= EVar v
-    Γ ::= [v]
-    l ::= [x]
-    ξ ::= v |-> EVar x
-
-Theorem subst_remove_scope_rev : forall e Γ ξ l,
-  (EXP Γ ++ l ⊢ subst ξ e -> forall vals, vals_subscoped vals Γ ->
-     EXP Γ ⊢ subst (ξ[[ ::= combine l vals]]) e) /\
-  (VAL Γ ++ l ⊢ subst ξ e -> forall vals, vals_subscoped vals Γ ->
-     VAL Γ ⊢ subst (ξ[[ ::= combine l vals]]) e).
-Proof.
-  induction e; intros; split; intros.
-  * constructor. constructor.
-  * constructor.
-  * constructor. simpl. simpl in H.
-Admitted. *)
-
-(* Fixpoint value_of_list (ξ : Substitution) (l : list VarFunId) : list Exp :=
-match l with
-| [] => []
-| x::xs => ξ x :: value_of_list ξ xs
-end.
-
-Theorem restrict_add :
-  forall l ξ, ξ = ((ξ -- l)[[::= combine l (value_of_list ξ l)]]).
-Proof.
-  (* unfold "--", extend_subst_list. *)
-  induction l; intros.
-  * simpl. reflexivity.
-  * unfold "--", extend_subst_list. simpl. extensionality v.
-    
-Admitted.
-
-Theorem alma : forall l Γ ξ,
-  subscoped l Γ ξ ->
-  vals_subscoped (value_of_list ξ l) Γ.
-Proof.
-Admitted. *)
-
-(*
-Does not hold, see previous counterexample:
-
-Theorem subst_remove_scope_rev : forall e Γ Γ' ξ l,
-  subscoped (Γ ++ l) Γ' ξ ->
-  (EXP Γ ++ l ⊢ subst (ξ -- l) e -> EXP Γ' ⊢ subst ξ e) /\
-  (VAL Γ ++ l ⊢ subst (ξ -- l) e -> VAL Γ' ⊢ subst ξ e).
-Proof.
-  
-Admitted.
-*)
-
-Theorem idsubst_restrict_is_idsubst :
-  forall l, idsubst -- l = idsubst.
-Proof.
-  intros. extensionality x. unfold "--". break_match_goal; auto.
-Qed.
-
-Hint Resolve idsubst_restrict_is_idsubst.
-
-Theorem idsubst_is_id_helper el :
-  Forall (fun e : Exp => subst idsubst e = e) el ->
-  map (subst idsubst) el = el.
-Proof.
-  induction el; auto.
-  simpl. intros. inversion H. subst. rewrite H2. rewrite IHel; auto. 
-Qed.
-
-Theorem idsubst_is_id :
-  forall e, subst idsubst e = e.
-Proof.
-  induction e using Exp_ind2 with
-    (Q := fun l => Forall (fun e => subst idsubst e = e) l); intros; simpl; auto.
-  * rewrite idsubst_restrict_is_idsubst, IHe. auto.
-  * rewrite idsubst_restrict_is_idsubst, IHe. auto.
-  * rewrite IHe, idsubst_is_id_helper; auto.
-  * rewrite idsubst_restrict_is_idsubst, IHe1, IHe2. auto.
-  * repeat rewrite idsubst_restrict_is_idsubst. rewrite IHe1, IHe2. auto.
-  * rewrite IHe1, IHe2. auto.
-  * rewrite IHe1, IHe2, IHe3. auto.
-Qed.
-
-Theorem idsubst_scoped :
-  forall Γ, subscoped Γ Γ idsubst.
-Proof.
-  intros. intro. intros. unfold idsubst. destruct v; constructor; auto.
-Qed.
-
-Hint Resolve idsubst_is_id.
-
-Theorem subst_preserves_scope_exp : forall e Γ,
-  (forall Γ' ξ,
-      subscoped Γ Γ' ξ -> EXP Γ' ⊢ subst ξ e) -> EXP Γ ⊢ e.
-Proof.
-  intros. specialize (H Γ idsubst (idsubst_scoped _)).
-  rewrite idsubst_is_id in H. auto.
-Qed.
-
-Theorem subst_preserves_scope_val : forall e Γ,
-  (forall Γ' ξ,
-      subscoped Γ Γ' ξ -> VAL Γ' ⊢ subst ξ e) -> VAL Γ ⊢ e.
-Proof.
-  intros. specialize (H Γ idsubst (idsubst_scoped _)).
-  rewrite idsubst_is_id in H. auto.
-Qed.
-
-
-Theorem subst_preserves_scope_rev : forall e Γ,
-  (EXP Γ ⊢ e ->
-    forall Γ' ξ,
-      subscoped Γ Γ' ξ -> EXP Γ' ⊢ subst ξ e) /\
-  (VAL Γ ⊢ e ->
-    forall Γ' ξ,
-      subscoped Γ Γ' ξ -> VAL Γ' ⊢ subst ξ e).
-Proof.
-  induction e using Exp_ind2 with (Q := 
-    fun l => Forall (fun e =>
-      forall Γ, (EXP Γ ⊢ e ->
-    forall Γ' ξ,
-      subscoped Γ Γ' ξ -> EXP Γ' ⊢ subst ξ e) /\
-  (VAL Γ ⊢ e ->
-    forall Γ' ξ,
-      subscoped Γ Γ' ξ -> VAL Γ' ⊢ subst ξ e)) l
-  ); try split; intros.
-
-(* LIT *)
-  * unfold subst. constructor. constructor.
-  * unfold subst. constructor.
-
-(* VAR *)
-  * inversion H. unfold subst. inversion H1. subst.
-    unfold subscoped in H0. constructor. apply H0. auto.
-  * inversion H. unfold subst. subst.
-    unfold subscoped in H0. apply H0. auto.
-
-(* FUNID *)
-  * inversion H. unfold subst. inversion H1. subst.
-    unfold subscoped in H0. constructor. apply H0. auto.
-  * inversion H. unfold subst. subst.
-    unfold subscoped in H0. apply H0. auto.
-
-(* FUN *)
-  * simpl. constructor. constructor. inversion H. inversion H1. subst.
-    eapply IHe; eauto. 
-  * simpl. constructor. inversion H. subst.
-    eapply IHe; eauto.
-
- (* RECFUN *)
-  * simpl. constructor. constructor. inversion H. inversion H1. subst.
-    eapply IHe; eauto. 
-  * simpl. constructor. inversion H. subst.
-    eapply IHe; eauto.
-
-(* APP *)
-  * simpl. inversion H. 2: inversion H1. subst. constructor.
-    - eapply IHe; eauto.
-    - intros. rewrite indexed_to_forall in IHe0. rewrite map_length in H1.
-      replace (ELit 0) with (subst ξ (ELit 0)) by reflexivity.
-      rewrite map_nth. eapply IHe0; eauto.
-  * inversion H.
-
-(* LET *)
-  * simpl. inversion H. subst. 2: inversion H1.
-    constructor; [ eapply IHe1 | eapply IHe2 ]; eauto.
-  * inversion H.
-
-(* LETREC *)
-  * simpl. inversion H. subst. 2: inversion H1.
-    constructor; [ eapply IHe1 | eapply IHe2 ]; eauto.
-  * inversion H.
-
-(* PLUS *)
-  * simpl. inversion H. subst. constructor; [ eapply IHe1 | eapply IHe2 ]; eauto.
-    inversion H1.
-  * inversion H.
-
-(* IF *)
-  * simpl. inversion H. subst. constructor; [ eapply IHe1 | eapply IHe2 | eapply IHe3 ]; eauto.
-    inversion H1.
-  * inversion H.
-
-(* APP HELPERS *)
-  * constructor. apply IHe. apply IHe0.
-  * constructor.
-Qed.
-
-
-
-
-
-
-(** Subst implies scope *)
-
-Definition partial_max (s1 s2 : Var) : string :=
-  if String.length s1 <? String.length s2 then s2 else s1
-.
-
-(** Just append an 's' to the front *)
-Definition string_succ (s : Var) : string := "s"%string ++ s.
-
-(** Maximum element of a list, with the custom max *)
-Definition list_max (l : list VarFunId) :=
-  fold_right (fun x acc => match x with
-                           | inl x' => partial_max x' acc
-                           | _      => acc
-                           end) EmptyString l.
-
-Definition new_fresh (l : list VarFunId) : Var :=
-  string_succ (list_max l).
-
-Theorem succ_neq_s : forall s, s <> string_succ s.
-Proof.
-  intro. intro. unfold string_succ in H. simpl in H. 
-  induction s; inversion H. subst. contradiction.
-Qed.
-
-Theorem max_not_in :
-  forall l s, partial_max (list_max l) s = s -> ~In (inl s) l.
-Proof.
-  induction l; intros.
-  * intro. inversion H0.
-  * intro. destruct (var_funid_eqb (inl s) a) eqn:P.
-    - apply var_funid_eqb_eq in P. subst.
-      simpl in H. unfold partial_max in H. break_match_hyp.
-      + break_match_hyp.
-        ** subst. apply Nat.ltb_lt in Heqb. apply Nat.ltb_lt in Heqb0. lia.
-        ** apply Nat.ltb_lt in Heqb. lia.
-      + break_match_hyp. congruence. admit.
-    - eapply IHl.
-Admitted.
-
-Theorem fresh_is_fresh :
-  forall l, ~In (inl (new_fresh l)) l.
-Proof.
-  intros. unfold new_fresh.
-  
-  intros. induction l; auto.
-  * simpl. intro.
-Admitted.
-
-Theorem app_in_not :
-  forall {T : Type} (l1 l2 : list T) x, ~In x (l1 ++ l2) -> ~In x l1 /\ ~In x l2.
-Proof.
-  intros. firstorder; intro; assert (In x (l1 ++ l2)). 
-  1, 3 : apply in_or_app; auto. all: congruence.
-Qed.
-
-(* Lemma magic_ξ_app_scope :
-  forall e Γ Γ' fresh p1 p2 l,
-  EXP Γ' ++ l ⊢ subst (magic_ξ Γ Γ' fresh p1 p2 -- l) e ->
-  exists fresh p1 p2, EXP Γ' ⊢ subst (magic_ξ (Γ ++ l) Γ' fresh p1 p2) e.
-Proof.
-  induction e; intros.
-  * exists (inl (new_fresh (Γ' ++ Γ ++ l0))).
-    pose (fresh_is_fresh (Γ' ++ Γ ++ l0)). apply app_in_not in n. destruct n.
-    exists H1, H0. simpl. constructor. constructor.
-  * 
-Admitted. *)
-
-Corollary in_app_left {T : Type} :
-  forall (l l' : list T) (x : T),
-  In x l -> In x (l ++ l').
-Proof.
-  firstorder. apply in_app_iff. auto.
-Qed.
-
-Corollary in_app_right {T : Type} :
-  forall (l l' : list T) (x : T),
-  In x l -> In x (l' ++ l).
-Proof.
-  firstorder. apply in_app_iff. auto.
-Qed.
-
-Module magic_ξ_gen.
-
-(* With fresh gen. *)
-Definition magic_ξ (Γ Γ' : list VarFunId)
-   : Substitution :=
-  fun x =>
-    if in_list x Γ then
-      if in_list x Γ'
-      then idsubst x
-      else ELit 0
-    else EVar (new_fresh (Γ ++ Γ')).
-
-Lemma magic_ξ_scope :
-  forall Γ Γ', subscoped Γ Γ' (magic_ξ Γ Γ').
-Proof.
-  intros. intro. intros. unfold magic_ξ. repeat break_match_goal.
-  * apply in_list_sound in Heqb. apply in_list_sound in Heqb0.
-    destruct v; constructor; auto.
-  * constructor.
-  * apply not_in_list_sound in Heqb. congruence.
-Qed.
-
-Lemma magic_ξ_app_scope :
-  forall Γ Γ' l,
-  magic_ξ Γ Γ' -- l = magic_ξ (Γ ++ l) (Γ' ++ l).
-Proof.
-  unfold "--", magic_ξ. intros.
-  extensionality x. repeat break_match_goal; auto.
-  * apply in_list_sound in Heqb. apply not_in_list_sound in Heqb1.
-    apply app_in_not in Heqb1. intuition.
-  * apply in_list_sound in Heqb. apply not_in_list_sound in Heqb0.
-    apply app_in_not in Heqb0. intuition.
-  * apply not_in_list_sound in Heqb3. apply in_list_sound in Heqb1.
-    apply app_in_not in Heqb3. intuition.
-  * apply in_list_sound in Heqb0. apply not_in_list_sound in Heqb2.
-    apply app_in_not in Heqb2. intuition.
-  * apply in_list_sound in Heqb3. apply not_in_list_sound in Heqb.
-    apply not_in_list_sound in Heqb1.
-    apply in_app_iff in Heqb3. intuition.
-  * apply not_in_list_sound in Heqb2. apply app_in_not in Heqb2.
-    apply in_list_sound in Heqb0. intuition.
-  * apply not_in_list_sound in Heqb. apply not_in_list_sound in Heqb0.
-    apply in_list_sound in Heqb1. apply in_app_iff in Heqb1. intuition.
-  * apply not_in_list_sound in Heqb. apply not_in_list_sound in Heqb0.
-    apply in_list_sound in Heqb1. apply in_app_iff in Heqb1. intuition.
-  * admit.
-Abort.
-
-Theorem magic_extend_restrict :
-  forall e Γ Γ' l,
-  (EXP Γ' ++ l ⊢ subst (magic_ξ Γ Γ' -- l) e -> EXP Γ' ++ l ⊢ subst (magic_ξ (Γ ++ l) (Γ' ++ l)) e) /\
-  (VAL Γ' ++ l ⊢ subst (magic_ξ Γ Γ' -- l) e -> VAL Γ' ++ l ⊢ subst (magic_ξ (Γ ++ l) (Γ' ++ l)) e).
-Proof.
-  induction e; intros; split; intros.
-  1-2: constructor. constructor.
-  * unfold magic_ξ, "--" in *. simpl in *. break_match_hyp.
-    - apply in_list_sound in Heqb.
-      eapply in_app_right with (l' := Γ) in Heqb as Heqb1.
-      eapply in_app_right with (l' := Γ') in Heqb as Heqb2.
-      apply in_list_sound in Heqb1. apply in_list_sound in Heqb2. rewrite Heqb1, Heqb2. auto.
-    - break_match_hyp.
-    2: {
-Abort.
-
-End magic_ξ_gen.
-
-Definition magic_ξ (Γ Γ' : list VarFunId) (name : VarFunId)
-   : Substitution :=
-  fun x =>
-    if in_list x Γ then
-      if in_list x Γ'
-      then idsubst x
-      else ELit 0
-    else idsubst name.
-
-Lemma magic_ξ_scope :
-  forall Γ Γ' name, subscoped Γ Γ' (magic_ξ Γ Γ' name).
-Proof.
-  intros. intro. intros. unfold magic_ξ. repeat break_match_goal.
-  * apply in_list_sound in Heqb. apply in_list_sound in Heqb0.
-    destruct v; constructor; auto.
-  * constructor.
-  * apply not_in_list_sound in Heqb. congruence.
-Qed.
-
-Theorem weaken_in {T : Type} : forall (l1 l2 l3 : list T) (x : T),
-  ~ In x ((l1 ++ l2) ++ l3 ++ l2) -> ~In x (l1 ++ l3).
-Proof.
-  intros. intro.
-  apply app_in_not in H. destruct H.
-  apply app_in_not in H. apply app_in_not in H1. destruct H, H1.
-  apply in_app_iff in H0. firstorder.
-Qed.
-
-Lemma magic_ξ_app_eq :
-  forall Γ Γ' l name,
-  magic_ξ Γ Γ' name -- l = magic_ξ (Γ ++ l) (Γ' ++ l) name.
-Proof.
-  unfold "--", magic_ξ. intros.
-  extensionality x. repeat break_match_goal; auto.
-  * apply in_list_sound in Heqb. apply not_in_list_sound in Heqb1.
-    apply app_in_not in Heqb1. intuition.
-  * apply in_list_sound in Heqb. apply not_in_list_sound in Heqb0.
-    apply app_in_not in Heqb0. intuition.
-  * apply not_in_list_sound in Heqb3. apply in_list_sound in Heqb1.
-    apply app_in_not in Heqb3. intuition.
-  * apply in_list_sound in Heqb0. apply not_in_list_sound in Heqb2.
-    apply app_in_not in Heqb2. intuition.
-  * apply in_list_sound in Heqb3. apply not_in_list_sound in Heqb.
-    apply not_in_list_sound in Heqb1.
-    apply in_app_iff in Heqb3. intuition.
-  * apply not_in_list_sound in Heqb2. apply app_in_not in Heqb2.
-    apply in_list_sound in Heqb0. intuition.
-  * apply not_in_list_sound in Heqb. apply not_in_list_sound in Heqb0.
-    apply in_list_sound in Heqb1. apply in_app_iff in Heqb1. intuition.
-  * apply not_in_list_sound in Heqb. apply not_in_list_sound in Heqb0.
-    apply in_list_sound in Heqb1. apply in_app_iff in Heqb1. intuition.
-Qed.
-
-Fixpoint names (e : Exp) : list VarFunId :=
-match e with
-| ELit l => []
-| EVar v => [inl v]
-| EFunId f => [inr f]
-| EFun vl e => map inl vl ++ names e
-| ERecFun f vl e => (inr f :: map inl vl) ++ names e
-| EApp exp l => names exp ++ flat_map names l
-| ELet v e1 e2 => [inl v] ++ names e1 ++ names e2 
-| ELetRec f vl b e => (inr f :: map inl vl) ++ names b ++ names e
-| EPlus e1 e2 => names e1 ++ names e2
-| EIf e1 e2 e3 => names e1 ++ names e2 ++ names e3
-end.
-
-Ltac app_in_not_tac :=
-match goal with
-| [ H : ~In _ (_ ++ _) |- _ ] => apply app_in_not in H
-end.
-
-
-(** Actually, this was not needed in the end, however it is useful to have it *)
-Lemma magic_ξ_name_irrelevant :
-  forall e, 
-  (forall Γ Γ' name, ~In name Γ -> ~In name Γ' -> ~In name (names e) ->
-  EXP Γ' ⊢ subst (magic_ξ Γ Γ' name) e ->
-  forall name', ~In name' Γ -> ~In name' Γ' -> ~In name' (names e) -> EXP Γ' ⊢ subst (magic_ξ Γ Γ' name') e) /\
-  (forall Γ Γ' name, ~In name Γ -> ~In name Γ' -> ~In name (names e) ->
-  VAL Γ' ⊢ subst (magic_ξ Γ Γ' name) e ->
-  forall name', ~In name' Γ -> ~In name' Γ' -> ~In name' (names e) -> VAL Γ' ⊢ subst (magic_ξ Γ Γ' name') e).
-Proof.
-  induction e using Exp_ind2 with
-  (Q := fun l => Forall (fun e => (forall Γ Γ' name, ~In name Γ -> ~In name Γ' -> ~In name (names e) ->
-  EXP Γ' ⊢ subst (magic_ξ Γ Γ' name) e ->
-  forall name', ~In name' Γ -> ~In name' Γ' -> ~In name' (names e) -> EXP Γ' ⊢ subst (magic_ξ Γ Γ' name') e) /\
-  (forall Γ Γ' name, ~In name Γ -> ~In name Γ' -> ~In name (names e) ->
-  VAL Γ' ⊢ subst (magic_ξ Γ Γ' name) e ->
-  forall name', ~In name' Γ -> ~In name' Γ' -> ~In name' (names e) -> VAL Γ' ⊢ subst (magic_ξ Γ Γ' name') e)) l)
-  ; try split; intros.
-  1-2: constructor. constructor.
-
-  (* VAR *)
-  * simpl. unfold magic_ξ in *. simpl in *. break_match_goal. break_match_goal.
-    - unfold idsubst. constructor. constructor. apply in_list_sound in Heqb0. auto.
-    - constructor. constructor.
-    - unfold idsubst in H2. destruct name; inversion H2; inversion H6; contradiction.
-  * simpl. unfold magic_ξ in *. simpl in *. break_match_goal. break_match_goal.
-    - unfold idsubst. constructor. apply in_list_sound in Heqb0. auto.
-    - constructor.
-    - unfold idsubst in H2. destruct name; inversion H2; inversion H6; subst; contradiction.
-
-  (* FUNID *)
-  * simpl. unfold magic_ξ in *. simpl in *. break_match_goal. break_match_goal.
-    - unfold idsubst. constructor. constructor. apply in_list_sound in Heqb0. auto.
-    - constructor. constructor.
-    - unfold idsubst in H2. destruct name; inversion H2; inversion H6; subst; contradiction.
-  * simpl. unfold magic_ξ in *. simpl in *. break_match_goal. break_match_goal.
-    - unfold idsubst. constructor. apply in_list_sound in Heqb0. auto.
-    - constructor.
-    - unfold idsubst in H2. destruct name; inversion H2; inversion H6; subst; contradiction.
-
-  (* FUN *)
-  * simpl subst in *. inversion H2. inversion H6. subst.
-    constructor. constructor. rewrite magic_ξ_app_eq in *.
-    destruct IHe. simpl in H1. apply app_in_not in H1. destruct H1.
-    simpl in H5. apply app_in_not in H5. destruct H5.
-    eapply H7. 4: exact H9. all: auto. all: apply app_not_in; auto. 
-  * simpl subst in *. inversion H2. subst.
-    constructor. rewrite magic_ξ_app_eq in *.
-    destruct IHe. simpl in H1. apply app_in_not in H1. destruct H1.
-    simpl in H5. apply app_in_not in H5. destruct H5.
-    eapply H6. 4: exact H7. all: auto. all: apply app_not_in; auto.
-
-  (* RECFUN *)
-  * simpl subst in *. inversion H2. inversion H6. subst.
-    constructor. constructor. rewrite magic_ξ_app_eq in *.
-    destruct IHe. apply app_in_not in H1. destruct H1.
-    apply app_in_not in H5. destruct H5. fold names in *. (* Coq oversimplifies names *)
-    eapply H7. 4: exact H9. all: auto. all: apply app_not_in; auto. 
-  * simpl subst in *. inversion H2. subst.
-    constructor. rewrite magic_ξ_app_eq in *.
-    destruct IHe. apply app_in_not in H1. destruct H1.
-    apply app_in_not in H5. destruct H5. fold names in *. (* Coq oversimplifies names *)
-    eapply H6. 4: exact H7. all: auto. all: apply app_not_in; auto. 
-
-  (* APP *)
-  * simpl in H1, H5. repeat app_in_not_tac. destruct H1, H5.
-    inversion H2. subst. simpl subst in *. constructor.
-    - eapply IHe. 4: exact H10. all: auto.
-    - intros. rewrite map_length in *. specialize (H11 i H8). rewrite indexed_to_forall in IHe0.
-      specialize (IHe0 i H8). destruct IHe0.
-      replace (ELit 0) with (subst (magic_ξ Γ Γ' name') (ELit 0)) by reflexivity.
-      replace (ELit 0) with (subst (magic_ξ Γ Γ' name) (ELit 0)) in H11 by reflexivity.
-      rewrite map_nth in *. eapply H9. 4: exact H11. all: auto.
-      apply notin_flat_map_Forall in H6. rewrite indexed_to_forall in H6. apply H6. auto.
-      apply notin_flat_map_Forall in H7. rewrite indexed_to_forall in H7. apply H7. auto.
-    - inversion H8.
-  * inversion H2.
-
-  (* LET *)
-  * simpl subst in *. inversion H2. subst. 
-    apply app_in_not in H1. apply app_in_not in H5. fold names in *. destruct H1, H5.
-    repeat app_in_not_tac. destruct H6, H7.
-    constructor.
-    - eapply IHe1. 4: exact H8. all: auto.
-    - rewrite magic_ξ_app_eq in *. eapply IHe2. 4: exact H10. all: try apply app_not_in. all: auto.
-    - inversion H6.
-  * inversion H2.
-
-  (* LETREC *)
-  * simpl subst in *. inversion H2. subst.
-    apply app_in_not in H1. apply app_in_not in H5. fold names in *. destruct H1, H5.
-    repeat app_in_not_tac. destruct H6, H7.
-    constructor.
-    - rewrite magic_ξ_app_eq in *. eapply IHe1. 4: exact H8. all: try apply app_not_in. all: auto.
-    - replace (inr f :: map inl vl) with ([inr f] ++ map inl vl) in * by reflexivity.
-      repeat app_in_not_tac. destruct H1, H5.
-      rewrite magic_ξ_app_eq in *. eapply IHe2. 4: exact H11. all: try apply app_not_in. all: auto.
-    - inversion H6.
-  * inversion H2.
-
-  (* PLUS *)
-  * simpl subst in *. inversion H2. subst. simpl in H5, H1. repeat app_in_not_tac. destruct H1, H5. 
-    constructor.
-    - eapply IHe1. 4: exact H8. all: eauto.
-    - eapply IHe2. 4: exact H9. all: eauto.
-    - inversion H6.
-  * inversion H2.
-
-  (* IF *)
-  * simpl subst in *. inversion H2. subst. 
-    simpl in H5, H1. repeat app_in_not_tac. destruct H1, H5.
-    repeat app_in_not_tac. destruct H6, H7.
-    constructor.
-    - eapply IHe1. 4: exact H9. all: eauto.
-    - eapply IHe2. 4: exact H10. all: eauto.
-    - eapply IHe3. 4: exact H11. all: eauto.
-    - inversion H6.
-  * inversion H2.
-  * constructor. eapply IHe. apply IHe0.
-  * constructor.
-Qed.
-
-Opaque app.
-
-Lemma magic_ξ_implies_scope : forall e Γ Γ' name 
-  (p1 : ~In name Γ) (p2 : ~In name Γ') (p3 : ~In name (names e)),
-  (EXP Γ' ⊢ subst (magic_ξ Γ Γ' name) e -> EXP Γ ⊢ e) /\
-  (VAL Γ' ⊢ subst (magic_ξ Γ Γ' name) e -> VAL Γ ⊢ e).
-Proof.
-  induction e using Exp_ind2 with
-  (Q := fun l => Forall (fun e => forall Γ Γ' name
-  (p1 : ~In name Γ) (p2 : ~In name Γ') (p3 : ~In name (names e)),
-    (EXP Γ' ⊢ subst (magic_ξ Γ Γ' name) e -> EXP Γ ⊢ e) /\
-    (VAL Γ' ⊢ subst (magic_ξ Γ Γ' name) e -> VAL Γ ⊢ e)
-  ) l); intros; try split; intros.
-  * constructor. constructor.
-  * constructor.
-  * constructor. constructor. simpl in H. unfold magic_ξ in H. repeat break_match_hyp.
-    - apply in_list_sound in Heqb. auto.
-    - apply in_list_sound in Heqb. auto.
-    - destruct name; inversion H; inversion H0; contradiction.
-  * constructor. simpl in H. unfold magic_ξ in H. repeat break_match_hyp.
-    - apply in_list_sound in Heqb. auto.
-    - apply in_list_sound in Heqb. auto.
-    - destruct name; inversion H; inversion H0; contradiction.
-  * constructor. constructor. simpl in H. unfold magic_ξ in H. repeat break_match_hyp.
-    - apply in_list_sound in Heqb. auto.
-    - apply in_list_sound in Heqb. auto.
-    - destruct name; inversion H; inversion H0; contradiction.
-  * constructor. simpl in H. unfold magic_ξ in H. repeat break_match_hyp.
-    - apply in_list_sound in Heqb. auto.
-    - apply in_list_sound in Heqb. auto.
-    - destruct name; inversion H; inversion H0; contradiction.
-  * constructor. constructor.
-    simpl in H. inversion H. inversion H0. subst.
-    erewrite magic_ξ_app_eq in H3. eapply (IHe _ (Γ' ++ map inl vl)). 4: exact H3. all: eauto.
-    all: try apply app_not_in; auto. all: apply app_in_not in p3; destruct p3; auto.
-  * constructor. simpl in H. inversion H. subst.
-    erewrite magic_ξ_app_eq in H1. eapply (IHe _ (Γ' ++ map inl vl)). 4: exact H1. all: eauto.
-    all: try apply app_not_in; auto. all: apply app_in_not in p3; destruct p3; auto.
-  * constructor. constructor.
-    simpl in H. inversion H. inversion H0. subst.
-    erewrite magic_ξ_app_eq in H3. eapply (IHe _ (Γ' ++ inr f :: map inl vl)). 4: exact H3. all: eauto.
-    all: try apply app_not_in; auto. all: apply app_in_not in p3; destruct p3; auto.
-  * constructor. simpl in H. inversion H. subst.
-    erewrite magic_ξ_app_eq in H1. eapply (IHe _ (Γ' ++ inr f :: map inl vl)). 4: exact H1. all: eauto.
-    all: try apply app_not_in; auto. all: apply app_in_not in p3; destruct p3; auto.
-  * inversion H. 2: inversion H0. subst. simpl in p3. app_in_not_tac. destruct p3.
-    apply notin_flat_map_Forall in H1. rewrite indexed_to_forall in IHe0, H1. constructor.
-    - eapply IHe. 4: exact H2. all: auto.
-    - intros. rewrite map_length in *. specialize (H3 i H4).
-      replace (ELit 0) with (subst (magic_ξ Γ Γ' name) (ELit 0)) in H3 by reflexivity.
-      rewrite map_nth in H3. eapply IHe0. 5: exact H3. all: auto.
-  * inversion H.
-  * inversion H. 2: inversion H0. subst. simpl names in p3. app_in_not_tac. destruct p3.
-    app_in_not_tac. destruct H1. constructor.
-    - eapply IHe1. 4: exact H2. all: auto.
-    - erewrite magic_ξ_app_eq in H4. eapply IHe2. 4: exact H4. all: try apply app_not_in; auto.
-  * inversion H.
-  * inversion H. 2: inversion H0. subst. simpl names in p3. app_in_not_tac. destruct p3.
-    app_in_not_tac. destruct H1. constructor.
-    - erewrite magic_ξ_app_eq in H2. eapply IHe1. 4: exact H2. all: try apply app_not_in; auto.
-    - erewrite magic_ξ_app_eq in H5.
-      replace (inr f :: map inl vl) with ([inr f] ++ map inl vl) in H0 by reflexivity. app_in_not_tac.
-      destruct H0. eapply IHe2. 4: exact H5. all: try apply app_not_in; auto.
-  * inversion H.
-  * inversion H. 2: inversion H0. subst. simpl in p3. app_in_not_tac. destruct p3.
-    constructor.
-    - eapply IHe1. 4: exact H2. all: auto.
-    - eapply IHe2. 4: exact H3. all: auto.
-  * inversion H.
-  * inversion H. 2: inversion H0. subst. simpl in p3. app_in_not_tac. destruct p3.
-    app_in_not_tac. destruct H1.
-    constructor.
-    - eapply IHe1. 4: exact H3. all: auto.
-    - eapply IHe2. 4: exact H4. all: auto.
-    - eapply IHe3. 4: exact H5. all: auto.
-  * inversion H.
-  * constructor. apply IHe. apply IHe0.
-  * constructor.
-Qed.
-
-Transparent app.
-
-Theorem sub_implies_scope_exp :
-  forall e Γ Γ',
-  (forall ξ, subscoped Γ Γ' ξ -> EXP Γ' ⊢ subst ξ e) -> EXP Γ ⊢ e.
-Proof.
-  intros. pose (fresh_is_fresh (Γ ++ Γ' ++ (names e))).
-  app_in_not_tac. destruct n. app_in_not_tac. destruct H1.
-  eapply magic_ξ_implies_scope with (name := inl (new_fresh (Γ ++ Γ' ++ (names e)))).
-  4: apply H; apply magic_ξ_scope.
-  all: auto.
-Qed.
-
-Lemma eval_list_length : forall l clock vl, eval_list (eval clock) l = Res vl -> length l = length vl.
-Proof.
-  induction l; intros.
-  * simpl in H. inversion H. auto.
-  * simpl in H. repeat break_match_hyp; try congruence. inversion H. simpl. erewrite IHl; eauto.
-Qed.
-
-Lemma eval_scoped_list l : forall v1 Γ clock,
-  (forall e v : Exp, eval clock e = Res v -> forall Γ : list VarFunId, EXP Γ ⊢ e -> VAL Γ ⊢ v) ->
-  (eval_list (eval clock) l = Res v1) ->
-  (forall i : nat, i < Datatypes.length l -> EXP Γ ⊢ nth i l (ELit 0))
-->
-  forall i : nat, i < length l -> VAL Γ ⊢ nth i v1 (ELit 0)
-  .
-Proof.
-  induction l; intros.
-  inversion H2. simpl in H0. repeat break_match_hyp; try congruence. inversion H0. subst.
-  destruct i.
-  * simpl. eapply H in Heqr; eauto. apply (H1 0). auto.
-  * simpl in H2. apply Lt.lt_S_n in H2. simpl. eapply IHl; eauto. intros. apply (H1 (S i0)). simpl. lia.
-Qed.
-
-Theorem extension_subscoped :
-  forall l ξ Γ Γ', subscoped Γ Γ' ξ -> forall vals, length vals = length l -> Forall (fun v => VAL Γ' ⊢ v) vals -> subscoped (Γ ++ l) Γ' (ξ[[::= combine l vals]]).
-Proof.
-  induction l; intros.
-  * cbn. rewrite app_nil_r. auto.
-  * apply eq_sym, element_exist in H0 as H0'. destruct H0', H2. subst.
-    cbn. replace ((fold_left (fun (ξ' : Substitution) '(x1, e) => ξ' [[x1 ::= e]]) (combine l x0) (ξ [[a ::= x]]))) with ((ξ[[ a ::= x ]]) [[ ::= combine l x0]]) by reflexivity. simpl in H0. inversion H0. inversion H1. subst.
-    epose (IHl (ξ[[a ::= x]]) (Γ ++ [a]) Γ' _ x0 (eq_sym H3) H6). rewrite <- app_assoc in s. simpl in s. auto.
-Unshelve.
-  unfold subscoped. intros. unfold extend_subst. break_match_goal.
-  - auto.
-  - apply H. apply in_app_iff in H2. destruct H2; auto. inversion H2; apply var_funid_eqb_neq in Heqb. congruence. inversion H4.
-Qed.
-
-Theorem eval_scoped_exp : forall clock e v,
-  eval clock e = Res v -> forall Γ, EXP Γ ⊢ e -> VAL Γ ⊢ v.
-Proof.
-  induction clock; intros. inversion H.
-  destruct e; inversion H; clear H; subst.
-  * constructor.
-  * inversion H0. auto.
-  * inversion H0. auto.
-  * repeat break_match_hyp; try congruence; subst.
-    - inversion H0. 2: inversion H. subst. eapply IHclock in H3. 2: eauto.
-      pose (eval_scoped_list _ _ _ _ IHclock Heqr0 H4).
-      inversion H3. subst. pose (subst_preserves_scope_rev e0 (Γ ++ map inl vl)). destruct a. clear H5.
-      specialize (H H1 Γ (idsubst [[ ::= combine (map inl vl) v1]])).
-      assert (subscoped (Γ ++ map inl vl) Γ (idsubst [[ ::= combine (map inl vl) v1]])). {
-        Search subscoped. apply extension_subscoped; auto. apply idsubst_scoped. rewrite map_length.
-        apply Nat.eqb_eq in Heqb. auto. rewrite Forall_nth. intros. apply Nat.eqb_eq in Heqb. 
-        apply eval_list_length in Heqr0 as H'. rewrite H' in v0.
-        specialize (v0 i H5). Search nth. erewrite nth_indep; eauto.
-      }
-      specialize (H H5). eapply IHclock; eauto.
-    - inversion H0. 2: inversion H. subst. eapply IHclock in H3. 2: eauto.
-      pose (eval_scoped_list _ _ _ _ IHclock Heqr0 H4).
-      inversion H3. subst. pose (subst_preserves_scope_rev e0 (Γ ++ inr f :: map inl vl)). destruct a. clear H5.
-      specialize (H H1 Γ (idsubst [[ ::= combine (inr f :: (map inl vl)) (ERecFun f vl e0 :: v1)]])).
-      assert (subscoped (Γ ++ inr f :: map inl vl) Γ (idsubst [[ ::= combine (inr f :: (map inl vl)) (ERecFun f vl e0 :: v1)]])). {
-        Search subscoped. apply extension_subscoped; auto. apply idsubst_scoped. simpl. rewrite map_length.
-        apply Nat.eqb_eq in Heqb. auto. rewrite Forall_nth. intros. apply Nat.eqb_eq in Heqb. 
-        apply eval_list_length in Heqr0 as H'. rewrite H' in v0. destruct i.
-        + simpl. auto.
-        + simpl in H5. apply Lt.lt_S_n in H5. specialize (v0 i H5). Search nth. erewrite nth_indep; eauto. simpl. lia.
-      }
-      specialize (H H5). eapply IHclock; eauto.
-  * break_match_hyp; try congruence.
-    inversion H0. 2: inversion H. subst.
-    pose (IHclock _ _ Heqr _ H3). pose (subst_preserves_scope_rev e2 (Γ ++ [inl v0])). destruct a.
-    clear H1. specialize (H H5 Γ (idsubst[[inl v0 ::= v1]])).
-    assert (subscoped (Γ ++ [inl v0]) Γ (idsubst [[inl v0 ::= v1]])).
-    { unfold subscoped. intros. unfold idsubst, extend_subst. break_match_goal.
-      - auto.
-      - destruct v3; constructor; apply in_app_iff in H1; destruct H1; auto.
-        all: apply var_funid_eqb_neq in Heqb; inversion H1; try congruence; inversion H4. }
-    specialize (H H1). eapply IHclock in H2; eauto.
-  * inversion H0. 2: inversion H. subst.
-    pose (subst_preserves_scope_rev e2 (Γ ++ [inr f])). destruct a. clear H1.
-    specialize (H H6 Γ (idsubst [[inr f ::= ERecFun f vl e1]])).
-    assert (subscoped (Γ ++ [inr f]) Γ (idsubst [[inr f ::= ERecFun f vl e1]])). {
-      unfold subscoped. intros. unfold idsubst, extend_subst. break_match_goal.
-      - constructor. auto.
-      - destruct v0; constructor; apply in_app_iff in H1; destruct H1; auto.
-        all: apply var_funid_eqb_neq in Heqb; inversion H1; try congruence; inversion H4.
-    }
-    specialize (H H1). eapply IHclock in H2; eauto.
-  * inversion H0. 2: inversion H. subst. repeat break_match_hyp; try congruence.
-    inversion H2. constructor.
-  * inversion H0. 2: inversion H. subst. break_match_hyp; try congruence. destruct v0. destruct l.
-    all: eapply IHclock in H2; eauto.
-Qed.
-
-(*
+(* FrameStack *)
+(** Based on Pitts' work: https://www.cl.cam.ac.uk/~amp12/papers/opespe/opespe-lncs.pdf *)
+(* Section stack_machine_semantics. *)
 Inductive Frame : Set :=
 | FApp1 (l : list Exp) (* apply □(e₁, e₂, ..., eₙ) *)
 | FApp2 (v : Exp) (p : is_value v) (l1 l2 : list Exp) (p2 : forall e, In e l2 -> is_value e) (** Can be problematic *)
-| FLet (v : Var) (e2 : Exp) (* let v = □ in e2 *)
+| FLet (e2 : Exp) (* let v = □ in e2 *)
 | FPlus1 (e2 : Exp) (* □ + e2 *)
 | FPlus2 (v : Exp) (p : is_value v) (* v + □ *)
 | FIf (e2 e3 : Exp) (* if □ then e2 else e3 *).
-*)
-(**
-  FrameStacks are closed, when all of their frames are closed.
-*)
+
+Definition FrameStack := list Frame.
+
+Lemma empty_is_value : forall e, In e [] -> is_value e. Proof. firstorder. Qed.
+Lemma step_value : forall l v,
+  (forall e, In e l -> is_value e) -> is_value v
+->
+  (forall e, In e (l ++ [v]) -> is_value e).
+Proof.
+  intros. apply in_app_or in H1. destruct H1.
+  * apply H. auto.
+  * firstorder. subst. auto.
+Qed.
+
 Inductive FCLOSED : FrameStack -> Prop :=
 | fclosed_nil : FCLOSED []
 | fclosed_app1 l xs:
@@ -1782,11 +877,11 @@ Inductive FCLOSED : FrameStack -> Prop :=
   FCLOSED xs
 ->
   FCLOSED (FApp2 v p l1 l2 p2::xs)
-| fclosed_let v e2 xs :
-  EXP [inl v] ⊢ e2 ->
+| fclosed_let e2 xs :
+  EXP 1 ⊢ e2 ->
   FCLOSED xs
 ->
-  FCLOSED (FLet v e2 :: xs)
+  FCLOSED (FLet e2 :: xs)
 | fclosed_plus1 e2 xs:
   EXPCLOSED e2 ->
   FCLOSED xs
@@ -1802,39 +897,3 @@ Inductive FCLOSED : FrameStack -> Prop :=
   FCLOSED xs
 ->
   FCLOSED (FIf e2 e3 :: xs).
-
-Theorem Forall_implies_subscoped vl : forall vals Γ ξ,
-  Forall (fun v => VAL Γ ⊢ v) vals -> length vl = length vals
-->
-  subscoped vl Γ (ξ[[::= combine vl vals]]).
-Proof.
-  induction vl; intros.
-  * apply eq_sym, length_zero_iff_nil in H0. subst. intro. intros. contradiction.
-  * apply element_exist in H0 as H0'. destruct H0', H1. subst.
-    intro. intros. cbn.
-    inversion H0. inversion H. subst. pose (IHvl _ _ (ξ[[a ::= x]]) H6 H3).
-    replace (fold_left (fun (ξ' : Substitution) '(x1, e) => ξ' [[x1 ::= e]]) (combine vl x0) (ξ [[a ::= x]])) with ((ξ [[a ::= x]])[[::= combine vl x0]]) by reflexivity. destruct (in_dec var_funid_eq_dec v vl).
-    + apply s. auto.
-    + erewrite subst_list_not_in; auto.  inversion H1. 2: contradiction. subst. inversion H. subst.
-      unfold extend_subst. rewrite var_funid_eqb_refl. apply H7.
-Qed.
-
-Theorem step_closedness : forall F e F' e',
-   ⟨ F, e ⟩ --> ⟨ F', e' ⟩ -> FCLOSED F -> EXPCLOSED e
-->
-  FCLOSED F' /\ EXPCLOSED e'.
-Proof.
-  intros F e F' e' IH. induction IH; intros.
-  * inversion H0. subst. inversion H4. subst. split; auto.
-    constructor; auto. destruct v; inversion H; inversion H1; auto.
-  * inversion H. inversion H0. subst. split; auto. inversion H5. exact H2.
-  * inversion H. inversion H0. subst. split; auto. inversion H5. subst. cbn in H2.
-    eapply subst_preserves_scope_rev; eauto. intro. intros. inversion H1. 2: contradiction.
-    subst. unfold idsubst, extend_subst. rewrite var_funid_eqb_refl. auto.
-  * inversion H0. subst. inversion H8. subst. split; auto. constructor; auto.
-    apply Forall_app. split; auto. constructor; auto. destruct v'; inversion H'; inversion H1; auto.
-  * inversion H3. subst. split; auto. inversion H9. eapply subst_preserves_scope_rev; eauto.
-    intro. intros. Search extend_subst_list. Search extend_subst.
-Qed.
-
-
